Checkpointing progress on map_secure

verified/kom_common.i.dfy
@@ -95,6 +95,16 @@ function monvaddr_page(mva:addr): PageNr
     (mva - KOM_DIRECTMAP_VBASE() - SecurePhysBase()) / PAGESIZE()
 }
 
+function paddr_page(p:addr): PageNr
+    requires PageAligned(p)
+    requires SecurePhysBase() <= p < SecurePhysBase() + KOM_SECURE_RESERVE()
+    ensures validPageNr(paddr_page(p))
+    ensures page_paddr(paddr_page(p)) == p
+{
+    (p - SecurePhysBase()) / PAGESIZE()
+}
+
+
 // workarounds for Spartan's lack of Dafny language features
 function specPageDb(t: (PageDb, int)): PageDb { t.0 }
 function specErr(t: (PageDb, int)): int { t.1 }
